theories/lang.v
@@ -51,6 +51,7 @@ Section nested_ind.
     | GenT (n: nat)
     | ExT (cname: tag) (* Ext C == ∃Ti, ClassT C Ti *)
     | DynamicT
+    | SupportDynT
   .
 
   Variable P : lang_ty -> Prop.
@@ -66,6 +67,7 @@ Section nested_ind.
   Hypothesis case_GenT: ∀ n, P (GenT n).
   Hypothesis case_ExT: ∀ cname, P (ExT cname).
   Hypothesis case_DynamicT : P DynamicT.
+  Hypothesis case_SupportDynT : P SupportDynT.
 
   Fixpoint lang_ty_ind (t : lang_ty) :=
     match t with
@@ -87,6 +89,7 @@ Section nested_ind.
     | GenT n => case_GenT n
     | ExT cname => case_ExT cname
     | DynamicT => case_DynamicT
+    | SupportDynT => case_SupportDynT
     end.
 End nested_ind.
 
@@ -110,6 +113,7 @@ Inductive bounded (n: nat) : lang_ty → Prop :=
   | NonNullIsBounded : bounded n NonNullT
   | ExIsBounded cname : bounded n (ExT cname)
   | DynamicIsBounded : bounded n DynamicT
+  | SupportDynIsBounded : bounded n SupportDynT
 .
 
 Global Hint Constructors bounded : core.
@@ -127,7 +131,7 @@ Fixpoint subst_ty (targs:list lang_ty) (ty: lang_ty):  lang_ty :=
 Corollary subst_ty_nil ty : subst_ty [] ty = ty.
 Proof.
   induction ty as [ | | | | cname targs hi | | | s t hs ht |
-      s t hs ht | n | cname | ] => //=.
+      s t hs ht | n | cname | | ] => //=.
   - f_equal.
     rewrite Forall_forall in hi.
     pattern targs at 2.
@@ -158,7 +162,7 @@ Lemma subst_ty_subst ty l k:
 Proof.
   move => hbounded.
   induction ty as [ | | | | cname targs hi | | | s t hs ht |
-      s t hs ht | n | cname | ] => //=.
+      s t hs ht | n | cname | | ] => //=.
   - f_equal.
     rewrite -list_fmap_compose.
     rewrite Forall_forall in hi.
@@ -213,7 +217,7 @@ Lemma bounded_subst n ty:
   bounded m (subst_ty targs ty).
 Proof.
   induction ty as [ | | | | cname targs hi | | | s t hs ht |
-      s t hs ht | k | cname | ] => //= hb m σ hlen hσ.
+      s t hs ht | k | cname | | ] => //= hb m σ hlen hσ.
   - constructor.
     rewrite Forall_forall => ty /elem_of_list_fmap hin.
     destruct hin as [ty' [-> hin]].
@@ -659,7 +663,7 @@ Lemma subst_ty_id n ty:
 Proof.
   move => h.
   induction ty as [ | | | | cname targs hi | | | s t hs ht |
-      s t hs ht | k | cname | ] => //=.
+      s t hs ht | k | cname | | ] => //=.
   - f_equal.
     rewrite Forall_forall in hi.
     pattern targs at 2.
