theories/progdef.v
@@ -37,6 +37,7 @@ Section ProgDef.
     | WfGen k: wf_ty (GenT k)
     | WfEx t : wf_ty (ExT t)
     | WfDynamic : wf_ty DynamicT
+    | WfSupportDyn : wf_ty SupportDynT
   .
 
   Hint Constructors wf_ty : core.
@@ -72,7 +73,7 @@ Section ProgDef.
   Proof.
     move => hwf.
     induction 1 as [ | | | | t targs def hdef hl h hi | | |
-        s t hs his ht hit | s t hs his ht hit | | | ] => //=; try (by constructor).
+        s t hs his ht hit | s t hs his ht hit | | | | ] => //=; try (by constructor).
     - econstructor; [ done | by rewrite map_length | ].
       move => k ty.
       rewrite list_lookup_fmap.
