theories/typing.v
@@ -38,6 +38,7 @@ Section Typing.
     | OkGen n: ok_ty Γ (GenT n)
     | OkEx t: ok_ty Γ (ExT t)
     | OkDynamic : ok_ty Γ DynamicT
+    | OkSupportDyn : ok_ty Γ SupportDynT
   .
 
   Lemma ok_ty_constraint_elim_ G T:
@@ -47,7 +48,7 @@ Section Typing.
     ok_ty Γ T.
   Proof.
     induction 1 as [ | | | | t σ def hσ hi hdef hconstr
-    | | | s t hs hi ht hit | s t hs hi ht hit | n | t | ] => Γ Γ' heq hΓ; subst; try by constructor.
+    | | | s t hs hi ht hit | s t hs hi ht hit | n | t | | ] => Γ Γ' heq hΓ; subst; try by constructor.
     - apply OkClass with def => //.
       + move => i ty h; by eapply hi.
       + move => i c h.
@@ -65,7 +66,7 @@ Section Typing.
   Lemma ok_ty_weaken Γ t: ok_ty Γ t → ∀ Γ', Γ ⊆ Γ' → ok_ty Γ' t.
   Proof.
     induction 1 as [ | | | | t σ def hσ hi hdef hconstr
-    | | | s t hs hi ht hit | s t hs hi ht hit | n | t | ] => Γ' hincl; try by constructor.
+    | | | s t hs hi ht hit | s t hs hi ht hit | n | t | | ] => Γ' hincl; try by constructor.
     - apply OkClass with def => //.
       + move => i ty h; by apply hi with i.
       + move => i c h.
@@ -93,7 +94,7 @@ Section Typing.
   Proof.
     move => hwp hcb.
     induction 1 as [ | | | | t σt def hσt hi hdef hconstr
-    | | | s t hs his ht hit | s t hs his ht hit | n | t | ]
+    | | | s t hs his ht hit | s t hs his ht hit | n | t | | ]
     => hwf Γ' σ hwfσ hokσ /=; try (constructor; by eauto).
     - apply OkClass with def => //.
       + move => i ty h.
@@ -172,7 +173,7 @@ Section Typing.
     ok_ty Γ' ty.
   Proof.
     induction 1 as [ | | | | t σ def hσ hi hdef hconstr
-    | | | s t hs hi ht hit | s t hs hi ht hit | n | t | ] => Γ' hΓ; try by constructor.
+    | | | s t hs hi ht hit | s t hs hi ht hit | n | t | | ] => Γ' hΓ; try by constructor.
     - econstructor => //.
       + move => k ty hk; by eauto.
       + move => k c' hc'.
